More progress in reorganization. This is still a broken commit.

SeparationLogic/Semantics/Down2Up.v
@@ -1,12 +1,19 @@
 Require Import Coq.Logic.Classical_Prop.
+Require Import Coq.Classes.RelationClasses.
+Require Import Coq.Relations.Relation_Definitions.
 Require Import Logic.lib.Coqlib.
-Require Import Logic.MinimunLogic.LogicBase.
+Require Import Logic.lib.Ensembles_ext.
+Require Import Logic.GeneralLogic.Base.
+Require Import Logic.MinimunLogic.Syntax.
 Require Import Logic.PropositionalLogic.Syntax.
 Require Import Logic.SeparationLogic.Syntax.
-Require Import Logic.PropositionalLogic.KripkeSemantics.
-Require Import Logic.SeparationLogic.SeparationAlgebra.
-Require Import Logic.SeparationLogic.SeparationAlgebraConstruction.
-Require Import Logic.SeparationLogic.Semantics. Import Logic.SeparationLogic.Semantics.DownwardsSemantics.
+Require Import Logic.PropositionalLogic.KripkeModel.
+Require Import Logic.SeparationLogic.Model.SeparationAlgebra.
+Require Import Logic.SeparationLogic.Model.OrderedSA.
+Require Import Logic.SeparationLogic.Model.UpwardsClosure.
+Require Import Logic.PropositionalLogic.Semantics.Kripke.
+Require Logic.SeparationLogic.Semantics.DownwardsSemantics.
+Require Logic.SeparationLogic.Semantics.FlatSemantics.
 
 Local Open Scope logic_base.
 Local Open Scope syntax.
@@ -16,9 +23,71 @@ Import SeparationLogicNotation.
 Import KripkeModelFamilyNotation.
 Import KripkeModelNotation_Intuitionistic.
 
-Module Downwards2Upwards.
+Module Down2Flat.
+Section Down2Flat.
 
-Definition dsSM {L: Language} {nL: NormalLanguage L} {pL: PropositionalLanguage L} {SL: SeparationLanguage L} {MD: Model} {kMD: KripkeModel MD} (M: Kmodel) {kiM: KripkeIntuitionisticModel (Kworlds M)} {J: Join  (Kworlds M)} {SA: SeparationAlgebra (Kworlds M)} {uSA: DownwardsClosedSeparationAlgebra (Kworlds M)} {SM: Semantics L MD} {kiSM: KripkeIntuitionisticSemantics L MD M SM} {dsSM: DownwardsSemantics L MD M SM}: @UpwardsSemantics.UpwardsSemantics L _ _ _ MD _ M kiM (UpwardsClosure_J) SM kiSM.
+Context {L: Language}
+        {nL: NormalLanguage L}
+        {pL: PropositionalLanguage L}
+        {sL: SeparationLanguage L}
+        {MD: Model}
+        {kMD: KripkeModel MD}
+        {M: Kmodel}
+        {R: Relation (Kworlds M)}
+        {kiM: KripkeIntuitionisticModel (Kworlds M)}
+        {J: Join  (Kworlds M)}
+        {SA: SeparationAlgebra (Kworlds M)}
+        {uSA: DownwardsClosedSeparationAlgebra (Kworlds M)}
+        {SM: Semantics L MD}
+        {kiSM: KripkeIntuitionisticSemantics L MD M SM}
+        {dsSM: DownwardsSemantics.SeparatingSemantics L MD M SM}.
+
+Definition fsSM: @FlatSemantics.SeparatingSemantics L _ MD _ M _ (UpwardsClosure_J) SM.
+Proof.
+  constructor.
+  + (* sat_sepcon *)
+    intros.
+    unfold WeakSemantics.sepcon.
+    split; unfold Included, Ensembles.In; intros m ?.
+    - rewrite (app_same_set (DownwardsSemantics.denote_sepcon _ _) m) in H.
+      destruct H as [m0 [m1 [m2 [? [? [? ?]]]]]].
+      exists m1, m2.
+      split; [| split]; auto.
+      exists m0; split; auto.
+    - rewrite (app_same_set (DownwardsSemantics.denote_sepcon _ _) m).
+      destruct H as [m1 [m2 [[n [? ?]] [? ?]]]].
+      exists n, m1, m2.
+      split; [| split; [| split]]; auto.
+  + (* sat_wand *)
+    intros.
+    unfold WeakSemantics.wand.
+    split; unfold Included, Ensembles.In; intros m ?.
+    - rewrite (app_same_set (DownwardsSemantics.denote_wand _ _) m) in H.
+      intros.
+      destruct H0 as [m2' [? ?]].
+      eapply sat_mono; eauto.
+      eapply H; eauto.
+    - rewrite (app_same_set (DownwardsSemantics.denote_wand _ _) m).
+      hnf; intros.
+      apply (H m1 m2); auto.
+      exists m2; split; auto.
+      reflexivity.
+Qed.
+
+Definition UsSM {s'L: SeparationEmpLanguage L} {USA: UnitalSeparationAlgebra (Kworlds M)} {deSM: DownwardsSemantics.EmpSemantics L MD M SM} : @FlatSemantics.EmpSemantics L _ _ MD _ M _ (UpwardsClosure_J) SM.
+Proof.
+  split; intros m; unfold Ensembles.In; unfold WeakSemantics.emp;
+  rewrite <- UpwardsClosure_increasing;
+  apply DownwardsSemantics.denote_emp.
+Qed.
+
+End Down2Flat.
+
+(*
+Module Downwards2Upwards.
+Section Downwards2Upwards.
+
+Definition dsSM : @UpwardsSemantics.UpwardsSemantics L _ _ _ MD _ M kiM (UpwardsClosure_J) SM kiSM.
 Proof.
   constructor.
   + (* sat_sepcon *)
@@ -57,43 +126,4 @@ Proof.
 Qed.
 
 End Downwards2Upwards.
-
-Module Downwards2Flat.
-
-Definition fsSM {L: Language} {nL: NormalLanguage L} {pL: PropositionalLanguage L} {SL: SeparationLanguage L} {MD: Model} {kMD: KripkeModel MD} (M: Kmodel) {kiM: KripkeIntuitionisticModel (Kworlds M)} {J: Join  (Kworlds M)} {SA: SeparationAlgebra (Kworlds M)} {uSA: DownwardsClosedSeparationAlgebra (Kworlds M)} {SM: Semantics L MD} {kiSM: KripkeIntuitionisticSemantics L MD M SM} {dsSM: DownwardsSemantics L MD M SM}: @FlatSemantics.FlatSemantics L _ _ _ MD _ M kiM (UpwardsClosure_J) SM kiSM.
-Proof.
-  constructor.
-  + (* sat_sepcon *)
-    intros.
-    pose proof Korder_PreOrder as H_PreOrder.
-    rewrite DownwardsSemantics.sat_sepcon.
-    split; intros.
-    - destruct H as [m0 [m1 [m2 [? [? [? ?]]]]]].
-      exists m1, m2.
-      split; [| split]; auto.
-      exists m0; split; auto.
-    - destruct H as [m1 [m2 [[n [? ?]] [? ?]]]].
-      exists n, m1, m2.
-      split; [| split; [| split]]; auto.
-  + (* sat_wand *)
-    intros.
-    pose proof Korder_PreOrder as H_PreOrder.
-    rewrite DownwardsSemantics.sat_wand.
-    simpl in *.
-    split; intros.
-    - destruct H0 as [m2' [? ?]].
-      eapply sat_mono; eauto.
-    - apply (H m1 m2); auto.
-      exists m2; split; auto.
-      reflexivity.
-Defined.
-
-Definition UsSM {L: Language} {nL: NormalLanguage L} {pL: PropositionalLanguage L} {SL: SeparationLanguage L} {uSL: UnitarySeparationLanguage L} {MD: Model} {kMD: KripkeModel MD} (M: Kmodel) {kiM: KripkeIntuitionisticModel (Kworlds M)} {J: Join  (Kworlds M)} {SA: SeparationAlgebra (Kworlds M)} {uSA: DownwardsClosedSeparationAlgebra (Kworlds M)} {USA: UnitalSeparationAlgebra (Kworlds M)} {SM: Semantics L MD} {kiSM: KripkeIntuitionisticSemantics L MD M SM} {dsSM: DownwardsSemantics L MD M SM} {UsSM: UnitalSemantics L MD M SM} : @UnitalSemantics L _ _ _ _ MD _ M kiM (UpwardsClosure_J) SM kiSM.
-Proof.
-  intros m; simpl.
-  rewrite <- UpwardsClosure_increasing.
-  apply sat_emp.
-Qed.
-
-End Downwards2Flat.
-
+*)
